refactor: change `Lets.WellTyped` to require the in and out context to be equal in the `nil` cast, rather than requiring just `ExtEq`

LeanMlirCommon/SimplyTyped/WellTyped.lean
@@ -73,7 +73,7 @@ def Expr.WellTyped (Γ : Context Ty) : UnTyped.Expr Op VarName → Ty → Prop
 
 /-- -/
 def Lets.WellTyped (Γ_in : Context Ty) : UnTyped.Lets Op VarName → Context Ty → Prop
-  | ⟨[]⟩, Γ_out       => Γ_out.ExtEq Γ_in
+  | ⟨[]⟩, Γ_out       => Γ_out = Γ_in -- Γ_out.ExtEq Γ_in
   | ⟨e :: es⟩, Γ_out  =>
       let eTy := (signature e.op).returnType
       Expr.WellTyped Γ_in e eTy ∧ Lets.WellTyped (Γ_in.push e.varName eTy) ⟨es⟩ Γ_out
@@ -155,27 +155,28 @@ theorem Lets.WellTyped.exists_iff {lets : UnTyped.Lets Op VarName} {Γ_in : Cont
 /-!
 ### Congr
 Show that well-typedness is preserved by extensionally equivalent contexts
+TODO: this is no longer true, now that we've switched `Lets.WellTyped` to use equality
 -/
 
-theorem Expr.WellTyped_of_extEq {Γ Δ : Context Ty} (e : UnTyped.Expr Op VarName)
-    (h_eq : Γ.ExtEq Δ) : Expr.WellTyped Γ e t → Expr.WellTyped Δ e t := by
-  intro h
-  rcases e
-  unfold WellTyped at h ⊢
-  simp at h ⊢
-  rcases h with ⟨h₁, h₂, h₃, rfl⟩
-  refine ⟨h₁, ?_, h₃, rfl⟩
-  intro ⟨v, ty⟩
-  sorry -- TODO: finish this proof
+-- theorem Expr.WellTyped_of_extEq {Γ Δ : Context Ty} (e : UnTyped.Expr Op VarName)
+--     (h_eq : Γ.ExtEq Δ) : Expr.WellTyped Γ e t → Expr.WellTyped Δ e t := by
+--   intro h
+--   rcases e
+--   unfold WellTyped at h ⊢
+--   simp at h ⊢
+--   rcases h with ⟨h₁, h₂, h₃, rfl⟩
+--   refine ⟨h₁, ?_, h₃, rfl⟩
+--   intro ⟨v, ty⟩
+--   sorry -- TODO: finish this proof
 
-theorem Lets.WellTyped_of_extEq {Γ_in Γ_out Δ_in Δ_out : Context Ty} {lets : UnTyped.Lets Op _}
-    (h_eq_in : Γ_in.ExtEq Δ_in) (h_eq_out : Γ_out.ExtEq Δ_out) :
-    Lets.WellTyped Γ_in lets Γ_out → Lets.WellTyped Δ_in lets Δ_out := by
-  intro h
-  rcases lets with ⟨lets⟩
-  induction lets
-  case nil =>
-    exact Context.ExtEq.trans h_eq_out.symm (Context.ExtEq.trans h h_eq_in)
-  case cons e lets ih =>
-    simp [WellTyped] at h ⊢
-    sorry -- TODO: finish
+-- theorem Lets.WellTyped_of_extEq {Γ_in Γ_out Δ_in Δ_out : Context Ty} {lets : UnTyped.Lets Op _}
+--     (h_eq_in : Γ_in.ExtEq Δ_in) (h_eq_out : Γ_out.ExtEq Δ_out) :
+--     Lets.WellTyped Γ_in lets Γ_out → Lets.WellTyped Δ_in lets Δ_out := by
+--   intro h
+--   rcases lets with ⟨lets⟩
+--   induction lets
+--   case nil =>
+--     exact Context.ExtEq.trans h_eq_out.symm (Context.ExtEq.trans h h_eq_in)
+--   case cons e lets ih =>
+--     simp [WellTyped] at h ⊢
+--     sorry -- TODO: finish
